From [[AS 1.3_1.]], [[DF 1.4_1.]] [[DF 1.4_2.]] [[CR 1.2_20.]] and [[CR 1.3_5.]] 
There exists an ES with a specific E$_x$ that is the case Now(E$_x$)
Because
Now(E$_x$)$\subset$Occurrence
it follows that
Occurrence(E$_x$)
Because it is a structural fact that E$_x$ is the case it follows
Happening(E$_x$)
(This experience E$_x$ is happening)
We say 
$\exists$ Happening(E$_x$)$\subseteq$SoE
and therefore the more general expression
Happening(x)$\subseteq$SoE and Occurrence$\subseteq$SoE
holds.
Since we concluded that 
Happening(E$_x$) $\land$ Now(E$_x$)
(Experience E$_x$ is happening and E$_x$ is in Now(x))
we can state that
Happening(Now(E$_x$))
This expierience is happening now
We reformulate 
ES = (S,SoE,CoE) 
as
ES =(S, E$_x$)
where
E$_x$ = (SoE(x), CoE(x))
We write
ES = (S, E$_x$) 
as
ES = (S, E(SoE(x),CoE(x)))
We can therefore say
$\exists$x such that for the adjusted form  it holds that
$\exists$ ES = (DS, E(Happening(Now(x)),CoE(x)))

